# 逻辑代数基本公式



|基本公式|
|-|
|$0 \cdot A = 0$|
|$1 \cdot A = A$|
|$A \cdot A = A$|
|$A \cdot A' = 0$|
|$A \cdot B = B \cdot A$|
|$A \cdot (B \cdot C) = (A \cdot B) \cdot C$|
|$A \cdot (B + C) = A \cdot B + A \cdot C$|
|$(A \cdot B)' = A' + B'$|
|$(A')' = A$|
|$1' = 0; 0' = 1$|
|$1 + A = 1$|
|$0 + A = A$|
|$A + A = A$|
|$A + A' = 1$|
|$A + B = B + A$|
|$A + (B + C) = (A + B) + C$|
|$A + B \cdot C = (A + B) \cdot (A + C)$，注意先逻辑与再逻辑或|
|$(A + B)' = A' \cdot B'$|

# 逻辑代数常用公式
|公式|
|-|
|$A + A \cdot B = A$|
|$A + A' \cdot B = A + B$|
|$A \cdot B + A \cdot B' = A$|
|$A \cdot (A + B) = A$|
|$A \cdot B + A' \cdot C + B \cdot C = A \cdot B + A' \cdot C$|
|$A \cdot B + A' \cdot C + BCD = A \cdot B + A' \cdot C$|
|$A \cdot (A \cdot B)' = A \cdot B'; A' \cdot (AB)' = A'$|
